$\left(2 \kappa_{2V}^{2} - 2 \kappa_{2V} \kappa_{V}^{2} - 3 \kappa_{2V} \kappa_{V} \kappa_{\lambda} + 3 \kappa_{V}^{3} \kappa_{\lambda}\right) \times \sigma{\left(\frac{1}{2},1,1 \right)} +$

$ \left(2 \kappa_{2V}^{2} - 2 \kappa_{2V} \kappa_{V}^{2} - \kappa_{2V} \kappa_{V} \kappa_{\lambda} + \kappa_{V}^{3} \kappa_{\lambda}\right) \times \sigma{\left(\frac{3}{2},1,1 \right)} +$

$ \left(- \frac{5 \kappa_{2V} \kappa_{V}^{2}}{4} + \frac{5 \kappa_{2V} \kappa_{V} \kappa_{\lambda}}{4} + \frac{\kappa_{V}^{3} \kappa_{\lambda}}{8} - \frac{\kappa_{V}^{2} \kappa_{\lambda}^{2}}{8}\right) \times \sigma{\left(1,2,1 \right)} +$

$ \left(- \kappa_{2V} \kappa_{V}^{2} + \kappa_{2V} \kappa_{V} \kappa_{\lambda} + \kappa_{V}^{4} - \kappa_{V}^{3} \kappa_{\lambda}\right) \times \sigma{\left(0,0,1 \right)} +$

$ \left(\frac{\kappa_{2V} \kappa_{V}^{2}}{36} - \frac{\kappa_{2V} \kappa_{V} \kappa_{\lambda}}{36} - \frac{\kappa_{V}^{3} \kappa_{\lambda}}{72} + \frac{\kappa_{V}^{2} \kappa_{\lambda}^{2}}{72}\right) \times \sigma{\left(1,10,1 \right)} +$

$ \left(- 4 \kappa_{2V}^{2} + \frac{56 \kappa_{2V} \kappa_{V}^{2}}{9} + \frac{16 \kappa_{2V} \kappa_{V} \kappa_{\lambda}}{9} - \frac{28 \kappa_{V}^{3} \kappa_{\lambda}}{9} + \frac{\kappa_{V}^{2} \kappa_{\lambda}^{2}}{9}\right) \times \sigma{\left(1,1,1 \right)}$
