$
A_{0} \left(- 2 \kappa_{2V}^{2} + \frac{9 \kappa_{2V} \kappa_{\lambda}}{4} + \frac{3 \kappa_{2V}}{4} - \kappa_{\lambda}^{2} - \frac{7 \kappa_{\lambda}}{4} + \frac{11}{4}\right) + A_{1} \left(\frac{\kappa_{2V} \kappa_{\lambda}}{2} - \frac{\kappa_{2V}}{2} - \frac{\kappa_{\lambda}}{2} + \frac{1}{2}\right) + A_{2} \left(\frac{2 \kappa_{2V}^{2}}{3} - \frac{5 \kappa_{2V} \kappa_{\lambda}}{3} + \frac{5 \kappa_{\lambda}}{3} - \frac{2}{3}\right) + A_{3} \left(\frac{4 \kappa_{2V}^{2}}{3} - \frac{4 \kappa_{2V} \kappa_{\lambda}}{3} + \frac{4 \kappa_{\lambda}}{3} - \frac{4}{3}\right) + A_{4} \left(\frac{2 \kappa_{2V} \kappa_{\lambda}}{5} - \frac{2 \kappa_{2V}}{5} + \frac{4 \kappa_{\lambda}^{2}}{5} - \frac{2 \kappa_{\lambda}}{5} - \frac{2}{5}\right) + A_{5} \left(- \frac{3 \kappa_{2V} \kappa_{\lambda}}{20} + \frac{3 \kappa_{2V}}{20} + \frac{\kappa_{\lambda}^{2}}{5} - \frac{7 \kappa_{\lambda}}{20} + \frac{3}{20}\right)
$
