$
A_{0} \left(2 \kappa_{2V}^{2} - \frac{124 \kappa_{2V} \kappa_{V}^{2}}{9} + \frac{61 \kappa_{2V} \kappa_{V} \kappa_{\lambda}}{9} + \frac{106 \kappa_{V}^{4}}{9} - \frac{17 \kappa_{V}^{3} \kappa_{\lambda}}{3} - \frac{\kappa_{V}^{2} \kappa_{\lambda}^{2}}{9}\right) + A_{1} \left(2 \kappa_{2V}^{2} - 8 \kappa_{2V} \kappa_{V}^{2} + 3 \kappa_{2V} \kappa_{V} \kappa_{\lambda} + 6 \kappa_{V}^{4} - 3 \kappa_{V}^{3} \kappa_{\lambda}\right) + A_{2} \left(- 4 \kappa_{2V}^{2} + 20 \kappa_{2V} \kappa_{V}^{2} - 8 \kappa_{2V} \kappa_{V} \kappa_{\lambda} - 16 \kappa_{V}^{4} + 8 \kappa_{V}^{3} \kappa_{\lambda}\right) + A_{3} \left(16 \kappa_{2V} \kappa_{V}^{2} - 16 \kappa_{2V} \kappa_{V} \kappa_{\lambda} - 16 \kappa_{V}^{4} + 16 \kappa_{V}^{3} \kappa_{\lambda}\right) + A_{4} \left(\frac{4 \kappa_{2V} \kappa_{V}^{2}}{5} - \frac{4 \kappa_{2V} \kappa_{V} \kappa_{\lambda}}{5} + \frac{\kappa_{V}^{4}}{5} - \frac{3 \kappa_{V}^{3} \kappa_{\lambda}}{10} + \frac{\kappa_{V}^{2} \kappa_{\lambda}^{2}}{10}\right) + A_{5} \left(- \frac{\kappa_{2V} \kappa_{V}^{2}}{45} + \frac{\kappa_{2V} \kappa_{V} \kappa_{\lambda}}{45} + \frac{\kappa_{V}^{4}}{45} - \frac{\kappa_{V}^{3} \kappa_{\lambda}}{30} + \frac{\kappa_{V}^{2} \kappa_{\lambda}^{2}}{90}\right)
$
