$
A_{0} \left(- 2 \kappa_{2V}^{2} + 6 \kappa_{2V} \kappa_{V}^{2} - 3 \kappa_{2V} \kappa_{V} \kappa_{\lambda} - 4 \kappa_{V}^{4} + 5 \kappa_{V}^{3} \kappa_{\lambda} - \kappa_{V}^{2} \kappa_{\lambda}^{2}\right) + A_{1} \left(- \frac{3 \kappa_{2V} \kappa_{V}^{2}}{2} + \frac{3 \kappa_{2V} \kappa_{V} \kappa_{\lambda}}{2} + \frac{5 \kappa_{V}^{4}}{2} - 3 \kappa_{V}^{3} \kappa_{\lambda} + \frac{\kappa_{V}^{2} \kappa_{\lambda}^{2}}{2}\right) + A_{2} \left(\frac{2 \kappa_{2V}^{2}}{3} - \frac{11 \kappa_{2V} \kappa_{V}^{2}}{6} + \frac{\kappa_{2V} \kappa_{V} \kappa_{\lambda}}{6} + \frac{7 \kappa_{V}^{4}}{6} - \frac{\kappa_{V}^{3} \kappa_{\lambda}}{6}\right) + A_{3} \left(\frac{4 \kappa_{2V}^{2}}{3} - \frac{8 \kappa_{2V} \kappa_{V}^{2}}{3} + \frac{4 \kappa_{2V} \kappa_{V} \kappa_{\lambda}}{3} + \frac{4 \kappa_{V}^{4}}{3} - \frac{4 \kappa_{V}^{3} \kappa_{\lambda}}{3}\right) + A_{4} \left(- \frac{\kappa_{2V} \kappa_{V}^{2}}{2} + \frac{\kappa_{2V} \kappa_{V} \kappa_{\lambda}}{2} + \frac{\kappa_{V}^{4}}{2} - \kappa_{V}^{3} \kappa_{\lambda} + \frac{\kappa_{V}^{2} \kappa_{\lambda}^{2}}{2}\right) + A_{5} \left(\frac{\kappa_{2V} \kappa_{V}^{2}}{2} - \frac{\kappa_{2V} \kappa_{V} \kappa_{\lambda}}{2} - \frac{\kappa_{V}^{4}}{2} + \frac{\kappa_{V}^{3} \kappa_{\lambda}}{2}\right)
$
